Starting proving correctness of translation.

Translation.v
@@ -17,33 +17,90 @@ Require ImpS.
 Module E := ImpE.
 Module S := ImpS.
 
-Function id_trans (md: E.mode) (c: S.com) : E.com :=
-  match c with
-  | S.Cskip => E.Cskip
-  | S.Cassign x e => E.Cassign x (id_trans_e md e)
-  | S.Cdeclassify x e => E.Cdeclassify x (id_trans_e md e)
-  | S.Cupdate e1 e2 => E.Cupdate (id_trans_e md e1) (id_trans_e md e2)
-  | S.Coutput e sl => E.Coutput (id_trans_e md e) sl
-  | S.Ccall e => E.Ccall (id_trans_e md e)
-  | S.Cset cnd => E.Cset cnd
-  | S.Cseq cs => E.Cseq (map (id_trans md) cs)
-  | S.Cif e c1 c2 => E.Cif (id_trans_e md e) (id_trans md c1) (id_trans md c2)
-  | S.Cwhile e c => E.Cwhile (id_trans_e md e) (id_trans md c)
-  end
+Module id_trans.
 
-with id_trans_e (md: E.mode) (e: S.exp) : E.exp :=
-  match e with
-  | S.Enat n => E.Enat n
-  | S.Evar x => E.Evar x
-  | S.Ebinop e1 e2 op => E.Ebinop (id_trans_e md e1) (id_trans_e md e2) op
-  | S.Eloc l => E.Eloc l
-  | S.Ederef e => E.Ederef (id_trans_e md e)
-  | S.Eisunset cnd => E.Eisunset cnd
-  | S.Elambda c => E.Elambda md (id_trans md c)
-  end.
+  Definition encl0 := 0.
+  Definition md := E.Encl encl0.
 
-Definition id_trans_wrapper (c: S.com) : E.com :=
-  E.Cenclave 0 (id_trans (E.Encl 0) c).
+  Definition rt_trans (rt: S.ref_type) : E.ref_type :=
+    match rt with
+    | S.Mut => E.Mut
+    | S.Immut => E.Immut
+    end.
+  
+  Fixpoint typ_trans (d: E.loc_mode) (s: S.base_type) : E.base_type :=
+    match s with
+    | S.Tnat => E.Tnat
+    | S.Tcond => E.Tcond md
+    | S.Tref (S.Typ s' p) rt =>
+      E.Tref (E.Typ (typ_trans d s') p) md (rt_trans rt)
+    | S.Tlambda Gminus U p Gplus =>
+      E.Tlambda (cntxt_trans d Gminus) [] U p md (cntxt_trans d Gplus) []
+    end
+
+  with cntxt_trans (d: E.loc_mode) (G: S.context) : E.context :=
+    match G with
+    | S.Cntxt vc lc =>
+      E.Cntxt
+        (fun x =>
+           match vc x with
+           | None => None
+           | Some (S.Typ s p) => Some (E.Typ (typ_trans d s) p)
+           end)
+        (fun l =>
+           match lc l with
+           | None => None
+           | Some (S.Typ s p, rt) => Some (E.Typ (typ_trans d s) p, rt_trans rt)
+           end)
+    end.
+  
+  Fixpoint id_trans (c: S.com) : E.com :=
+    match c with
+    | S.Cskip => E.Cskip
+    | S.Cassign x e => E.Cassign x (id_trans_e e)
+    | S.Cdeclassify x e => E.Cdeclassify x (id_trans_e e)
+    | S.Cupdate e1 e2 => E.Cupdate (id_trans_e e1) (id_trans_e e2)
+    | S.Coutput e sl => E.Coutput (id_trans_e e) sl
+    | S.Ccall e => E.Ccall (id_trans_e e)
+    | S.Cset cnd => E.Cset cnd
+    | S.Cseq cs => E.Cseq (map id_trans cs)
+    | S.Cif e c1 c2 => E.Cif (id_trans_e e) (id_trans c1) (id_trans c2)
+    | S.Cwhile e c => E.Cwhile (id_trans_e e) (id_trans c)
+    end
+
+  with id_trans_e (e: S.exp) : E.exp :=
+    match e with
+    | S.Enat n => E.Enat n
+    | S.Evar x => E.Evar x
+    | S.Ebinop e1 e2 op => E.Ebinop (id_trans_e e1) (id_trans_e e2) op
+    | S.Eloc l => E.Eloc l
+    | S.Ederef e => E.Ederef (id_trans_e e)
+    | S.Eisunset cnd => E.Eisunset cnd
+    | S.Elambda c => E.Elambda md (id_trans c)
+    end.
+
+  Definition id_trans_wrapper (c: S.com) : E.com :=
+    E.Cenclave encl0 (id_trans c).
+
+  Hint Constructors E.exp_type E.com_type.
+  
+  Lemma id_trans_sound' (c: S.com) (d: E.loc_mode) :
+    forall pc G U G',
+      S.com_wt pc G U c G' ->
+      E.com_type pc md (cntxt_trans d G) [] U d (id_trans c)
+                 (cntxt_trans d G') [].
+  Proof.
+    induction c using S.com_ind' with
+    (P0:=fun e => forall G s p,
+             S.exp_wt G e (S.Typ s p) ->
+             E.exp_type md (cntxt_trans d G) d (id_trans_e e)
+                        (E.Typ (typ_trans d s) p)).
+    - intros. inversion H. subst. simpl. apply E.ETnat.
+    - intros. inversion H. subst. simpl. apply E.ETvar.
+      destruct G. simpl in *. now rewrite H2.
+    - intros. inversion H. subst. simpl.
+      apply E.ETbinop; [apply IHc in H3 | apply IHc0 in H7]; auto.
+    - intros. inversion H. subst. simpl. constructor. Focus 2. subst.
 
 (*
 Lemma id_trans_ind:
@@ -57,4 +114,6 @@ Proof.
   intros.
   induction c using S.com_ind' with (P0:=fun e => P0 md e (id_trans_e md e)).
   Focus 9. simpl. auto.
-  *)
+ *)
+
+End id_trans.
